src/Narcissus/Automation/NormalizeFormats.v
@@ -160,7 +160,8 @@ Ltac normalize_step BitStringT :=
          | eapply EquivFormat_trans; [apply EquivFormat_If_Then_Else with (monoid := BitStringT) | ]
          | apply EquivFormat_If_Then_Else_Proper
          | eapply (@EquivFormat_UnderSequence _ _ BitStringT)
-         | eapply EquivFormat_Projection_Format_Empty_Format]; intros).
+         | eapply EquivFormat_Projection_Format_Empty_Format
+         | unfold EquivFormat; intros; reflexivity]; intros).
 
 Ltac normalize_format :=
   (* Normalize formats by performing algebraic simplification. *)
