src/Narcissus/Formats/Option.v
@@ -115,4 +115,67 @@ Proof.
   }
 Qed.
 
+  Lemma option_format_correct'
+      {P  : CacheDecode -> Prop}
+      {P_invT P_invE : (CacheDecode -> Prop) -> Prop}
+      (P_inv_pf : cache_inv_Property P (fun P => P_invT P /\ P_invE P))
+      (predicate_Some : S -> Prop)
+      (predicate_None : () -> Prop)
+      (b' : bool)
+      (predicate :=
+         fun a_opt =>
+           decides (negb b') (a_opt = None)
+           /\ match a_opt with
+              | Some a => predicate_Some a
+              | None => predicate_None ()
+              end)
+      (format_Some : FormatM S T)
+      (format_None : FormatM () T)
+      (decode_Some : DecodeM (S * T) T)
+      (decode_None : DecodeM (() * T) T)
+      (decode_Some_pf :
+         cache_inv_Property P P_invT
+         -> CorrectDecoder
+              monoid predicate_Some (fun _ _ => True)
+              format_Some decode_Some P)
+      (decode_None_pf :
+         cache_inv_Property P P_invE
+         -> CorrectDecoder
+              monoid predicate_None (fun _ _ => True)
+              format_None decode_None P)
+  : CorrectDecoder
+      monoid
+      predicate
+      (fun _ _ => True)
+      (format_option format_Some format_None)%comp
+      (option_decode decode_Some decode_None b')
+ P.
+Proof.
+  unfold cache_inv_Property in *; split.
+  { intros env env' xenv data bin ext ? env_pm pred_pm pred_pm_rest com_pf.
+    unfold format_option in com_pf; computes_to_inv;
+      unfold option_decode; destruct data;
+      find_if_inside; unfold predicate in *; simpl in *;
+        intuition; try discriminate.
+    - eapply H3 in com_pf; destruct_ex;
+        intuition eauto; rewrite H6; eauto.
+    - eapply H4 in com_pf; destruct_ex;
+        intuition eauto; rewrite H6; eauto.
+  }
+  { unfold option_decode; intros.
+    find_if_inside; simpl in *.
+    - destruct (decode_Some bin env') as [ [ [? ?] ?] | ] eqn : ? ;
+        simpl in *; try discriminate; injections; simpl.
+      eapply decode_Some_pf in Heqo; intuition eauto.
+      destruct_ex; intuition; subst.
+      eexists _; eexists _; unfold predicate; intuition eauto.
+      discriminate.
+    - destruct (decode_None bin env') as [ [ [? ?] ?] | ] eqn : ? ;
+        simpl in *; try discriminate; injections; destruct u.
+      eapply decode_None_pf in Heqo; intuition eauto; destruct_ex;
+        intuition eauto; subst.
+      eexists _; eexists _; unfold predicate; intuition eauto.
+  }
+Qed.
+
 End Option.
